tidy up normalization + start of unscoped level one

theories/LevelOneScoped.v
@@ -1,7 +1,7 @@
 From Prototype Require Import Prelude Sig.
 
-(** This file defines terms and substitutions over an abstract signature.
-    Substitutions are represented as functions [nat -> term],
+(** This file defines exprs and substitutions over an abstract signature.
+    Substitutions are represented as functions [fin n -> term m],
     and we prove the main properties of substitution. *)
 
 Module Make (S : Sig).
@@ -14,29 +14,38 @@ Definition arg_ty := @arg_ty (base S.t).
 (** Terms are indexed by (meta-level) kinds. *)
 Inductive kind := 
 | (** Term. *)
-  K_t : kind
+  Kt : kind
 | (** Constructor argument. *)
-  K_a : arg_ty -> kind
+  Ka : arg_ty -> kind
 | (** List of constructor arguments. *)
-  K_al : list arg_ty -> kind.
+  Kal : list arg_ty -> kind.
+Derive NoConfusion for kind.
+
+(** Notations for expressions with known kinds. *)
+Reserved Notation "'term' n" (at level 0).
+Reserved Notation "'arg' ty n" (at level 0, ty at level 0).
+Reserved Notation "'args' tys n" (at level 0, tys at level 0).
 
 (** Terms over an abstract signature. 
     Terms are indexed by a kind and a scope (a natural). *)
-Inductive term : kind -> nat -> Type :=
+Inductive expr : kind -> nat -> Type :=
 | (** Term variable. *)
-  T_var {n} : fin n -> term K_t n
-| (** Non-variable term constructor, applied to a list of arguments. *)
-  T_ctor {n} : forall c, term (K_al (ctor_type S.t c)) n -> term K_t n
+  T_var {n} : fin n -> term n
+| (** Non-variable expr constructor, applied to a list of arguments. *)
+  T_ctor {n} : forall c, args (ctor_type S.t c) n -> term n
 | (** Empty argument list. *)
-  T_al_nil {n} : term (K_al []) n
+  T_al_nil {n} : args [] n
 | (** Non-empty argument list. *)
-  T_al_cons {n ty tys} : term (K_a ty) n -> term (K_al tys) n -> term (K_al (ty :: tys)) n
+  T_al_cons {n ty tys} : arg ty n -> args tys n -> args (ty :: tys) n
 | (** Base argument (e.g. bool or string). *)
-  T_abase {n} : forall b, denote_base S.t b -> term (K_a (AT_base b)) n
+  T_abase {n} : forall b, denote_base S.t b -> arg (AT_base b) n
 | (** Term argument. *)
-  T_aterm {n} : term K_t n -> term (K_a AT_term) n
+  T_aterm {n} : term n -> arg AT_term n
 | (** Binder argument. *)
-  T_abind {n ty} : term (K_a ty) (S n) -> term (K_a (AT_bind ty)) n.
+  T_abind {n ty} : arg ty (S n) -> arg (AT_bind ty) n
+where "'term' n" := (expr Kt n)
+  and "'arg' ty n" := (expr (Ka ty) n)
+  and "'args' tys n" := (expr (Kal tys) n).
 
 (*********************************************************************************)
 (** *** Renamings. *)
@@ -59,38 +68,31 @@ Equations rcons {n m} (i0 : fin m) (r : ren n m) : ren (S n) m :=
 rcons i0 _ fin_zero := i0 ;
 rcons i0 r (fin_succ i) := r i.
 
-(*#[global] Instance rcons_notation n m : Scons (fin m) (ren n m) (ren (S n) m) :=
-{ gen_scons := @rcons n m }.*)
-
 (** Compose two renamings (left to right composition). *)
 Equations rcomp {n m o} (r1 : ren n m) (r2 : ren m o) : ren n o :=
 rcomp r1 r2 i := r2 (r1 i).
-(*#[global] Instance rcomp_notation {n m o} : Scomp (ren n m) (ren m o) (ren n o) :=
-{ gen_scomp := rcomp }.*)
 
 (** Lift a renaming through a binder. *)
 Equations up_ren {n m} (r : ren n m) : ren (S n) (S m) := 
 up_ren r := rcons fin_zero (rcomp r (rshift 1)).
  
-(** Rename a term. *)
-Equations rename {n m} {k} (t : term k n) (r : ren n m) : term k m :=
+(** Rename a expr. *)
+Equations rename {n m} {k} (t : expr k n) (r : ren n m) : expr k m :=
 rename (T_var i) r := T_var (r i) ;
-rename (T_ctor c args) r := T_ctor c (rename args r) ;
+rename (T_ctor c al) r := T_ctor c (rename al r) ;
 rename T_al_nil r := T_al_nil ;
-rename (T_al_cons a args) r := T_al_cons (rename a r) (rename args r) ;
+rename (T_al_cons a al) r := T_al_cons (rename a r) (rename al r) ;
 rename (T_abase b x) r := T_abase b x ;
 rename (T_aterm t) r := T_aterm (rename t r) ;
 rename (T_abind a) r := T_abind (rename a (up_ren r)).
-(*#[global] Instance rename_notation n m k : Subst (term k n) (ren n m) (term k m) :=
-{ gen_subst := rename }.*)
-  
+
 (*********************************************************************************)
 (** *** Substitutions. *)
 (*********************************************************************************)
 
-(** A substitution on terms is a function [fin n -> term K_t m] which is applied 
+(** A substitution on terms is a function [fin n -> term m] which is applied 
     to all free variables. *)
-Definition subst n m := fin n -> term K_t m.
+Definition subst n m := fin n -> term m.
 
 (** The identity substitution. *)
 Equations sid {n} : subst n n := 
@@ -101,33 +103,27 @@ Equations sshift {n} (k : nat) : subst n (k + n) :=
 sshift k i := T_var (fin_weaken k i).
 
 (** Cons a term with a substitution. *)
-Equations scons {n m} (t : term K_t m) (s : subst n m) : subst (S n) m :=
+Equations scons {n m} (t : term m) (s : subst n m) : subst (S n) m :=
 scons t s fin_zero := t ;
 scons t s (fin_succ i) := s i.
-(*#[global] Instance scons_notation n m : Scons (term K_t m) (subst n m) (subst (S n) m) :=
-{ gen_scons := scons }.*)
 
 (** Lift a substitution through a binder. *)
 Equations up_subst {n m} (s : subst n m) : subst (S n) (S m) :=
 up_subst s := scons (T_var fin_zero) (fun i => rename (s i) (rshift 1)).
 
 (** Apply a substitution to a term. *)
-Equations substitute {n m} {k} (t : term k n) (s : subst n m) : term k m :=
+Equations substitute {n m} {k} (t : expr k n) (s : subst n m) : expr k m :=
 substitute (T_var i) s := s i ;
-substitute (T_ctor c args) s := T_ctor c (substitute args s) ;
+substitute (T_ctor c al) s := T_ctor c (substitute al s) ;
 substitute T_al_nil s := T_al_nil ;
-substitute (T_al_cons a args) s := T_al_cons (substitute a s) (substitute args s) ;
+substitute (T_al_cons a al) s := T_al_cons (substitute a s) (substitute al s) ;
 substitute (T_abase b x) s := T_abase b x ;
 substitute (T_aterm t) s := T_aterm (substitute t s) ;
 substitute (T_abind a) s := T_abind (substitute a (up_subst s)).
-(*#[global] Instance substitute_notation n m k : Subst (term k n) (subst n m) (term k m) :=
-{ gen_subst := substitute }.*)
 
 (** Left to right composition of substitutions. *)
 Equations scomp {n m o} (s1 : subst n m) (s2 : subst m o) : subst n o :=
 scomp s1 s2 i := substitute (s1 i) s2.
-(*#[global] Instance scomp_notation n m o : Scomp (subst n m) (subst m o) (subst n o) :=
-{ gen_scomp := scomp }.*)
 
 (*********************************************************************************)
 (** *** Setoid Rewrite Support. *)
@@ -195,14 +191,14 @@ Lemma up_ren_comp {n m o} (r1 : ren n m) (r2 : ren m o) :
   rcomp (up_ren r1) (up_ren r2) =₁ up_ren (rcomp r1 r2).
 Proof. intros i. dependent elimination i ; reflexivity. Qed.  
 
-Lemma ren_ren {n m o k} (t : term k n) (r1 : ren n m) (r2 : ren m o) : 
+Lemma ren_ren {n m o k} (t : expr k n) (r1 : ren n m) (r2 : ren m o) : 
   rename (rename t r1) r2 = rename t (rcomp r1 r2).
 Proof.
 funelim (rename t _) ; simp rename in * ; auto.
 now rewrite H, up_ren_comp.
 Qed.
 
-Lemma subst_ren {n m o k} (t : term k n) (s : subst n m) (r : ren m o) : 
+Lemma subst_ren {n m o k} (t : expr k n) (s : subst n m) (r : ren m o) : 
   rename (substitute t s) r = substitute t (fun i => rename (s i) r).
 Proof.
 funelim (substitute t _) ; simp rename substitute in * ; auto.
@@ -212,7 +208,7 @@ rewrite ren_ren, ren_ren. apply rename_proper ; auto.
 reflexivity.
 Qed.
 
-Lemma ren_subst {n m o k} (t : term k n) (r : ren n m) (s : subst m o) : 
+Lemma ren_subst {n m o k} (t : expr k n) (r : ren n m) (s : subst m o) : 
   substitute (rename t r) s = substitute t (fun i => s (r i)).
 Proof.
 funelim (rename t r) ; simp rename substitute in * ; auto.
@@ -228,7 +224,7 @@ rewrite ren_subst, subst_ren. apply substitute_proper ; auto.
 intros i. simp scons rshift fin_weaken. reflexivity.
 Qed.
 
-Lemma subst_subst {n m o k} (t : term k n) (s1 : subst n m) (s2 : subst m o) : 
+Lemma subst_subst {n m o k} (t : expr k n) (s1 : subst n m) (s2 : subst m o) : 
   substitute (substitute t s1) s2 = substitute t (scomp s1 s2).
 Proof.
 funelim (substitute t _) ; simp substitute in * ; auto.
@@ -239,7 +235,7 @@ Lemma up_subst_sid {n} : (up_subst (@sid n)) =₁ sid.
 Proof. intros i ; dependent elimination i ; reflexivity. Qed.
 #[global] Hint Rewrite @up_subst_sid : up_subst.
 
-Lemma subst_sid {n k} (t : term n k) : substitute t sid = t.
+Lemma subst_sid {n k} (t : expr n k) : substitute t sid = t.
 Proof.
 induction t ; simp substitute in * ; auto.
 rewrite up_subst_sid. auto.
@@ -258,7 +254,7 @@ Lemma scomp_assoc {n m o p} (s1 : subst n m) (s2 : subst m o) (s3 : subst o p) :
   scomp (scomp s1 s2) s3 =₁ scomp s1 (scomp s2 s3).
 Proof. intros i. simp scomp. now rewrite subst_subst. Qed.
 
-Lemma ren_is_subst {n m k} (t : term k n) (r : ren n m) : 
+Lemma ren_is_subst {n m k} (t : expr k n) (r : ren n m) : 
   rename t r = substitute t (fun i => T_var (r i)).
 Proof.
 funelim (rename t r) ; simp rename substitute in * ; auto.
@@ -266,7 +262,7 @@ f_equal. rewrite H. apply substitute_proper ; auto.
 intros i. dependent elimination i ; reflexivity.
 Qed.
 
-Lemma rshift_sshift {n k} (t : term k n) : 
+Lemma rshift_sshift {n k} (t : expr k n) : 
   rename t (rshift 1) = substitute t (sshift 1).
 Proof. rewrite ren_is_subst. reflexivity. Qed.
     
@@ -284,7 +280,7 @@ Lemma sid_scons {n} : scons (T_var fin_zero) (sshift 1) =₁ @sid (S n).
 Proof. intros i. dependent elimination i ; reflexivity. Qed.
 #[global] Hint Rewrite @sid_scons : scons.
 
-Lemma scomp_scons_distrib {n m o} (t : term K_t m) (s1 : subst n m) (s2 : subst m o) :
+Lemma scomp_scons_distrib {n m o} (t : term m) (s1 : subst n m) (s2 : subst m o) :
   scomp (scons t s1) s2 =₁ scons (substitute t s2) (scomp s1 s2).
 Proof. intros i. dependent elimination i ; reflexivity. Qed.
 
