theories/LevelOneUnscoped.v
@@ -1,0 +1,284 @@
+From Prototype Require Import Prelude Sig.
+
+(** This file defines exprs and substitutions over an abstract signature.
+    Substitutions are represented as functions [nat -> term],
+    and we prove the main properties of substitution. *)
+
+Module Make (S : Sig).
+Definition arg_ty := @arg_ty (base S.t).
+
+(*********************************************************************************)
+(** *** Terms. *)
+(*********************************************************************************)
+
+(** Terms are indexed by (meta-level) kinds. *)
+Inductive kind := 
+| (** Term. *)
+  Kt : kind
+| (** Constructor argument. *)
+  Ka : arg_ty -> kind
+| (** List of constructor arguments. *)
+  Kal : list arg_ty -> kind.
+Derive NoConfusion for kind.
+
+(** Notations for expressions with known kinds. *)
+Reserved Notation "'term'" (at level 0).
+Reserved Notation "'arg' ty" (at level 0, ty at level 0).
+Reserved Notation "'args' tys" (at level 0, tys at level 0).
+
+(** Terms over an abstract signature. 
+    Terms are indexed by a kind. *)
+Inductive expr : kind -> Type :=
+| (** Term variable. *)
+  T_var : nat -> term
+| (** Non-variable expr constructor, applied to a list of arguments. *)
+  T_ctor : forall c, args (ctor_type S.t c) -> term
+| (** Empty argument list. *)
+  T_al_nil : args []
+| (** Non-empty argument list. *)
+  T_al_cons {ty tys} : arg ty -> args tys -> args (ty :: tys)
+| (** Base argument (e.g. bool or string). *)
+  T_abase : forall b, denote_base S.t b -> arg (AT_base b)
+| (** Term argument. *)
+  T_aterm : term -> arg AT_term
+| (** Binder argument. *)
+  T_abind {ty} : arg ty -> arg (AT_bind ty)
+where "'term'" := (expr Kt)
+  and "'arg' ty" := (expr (Ka ty))
+  and "'args' tys" := (expr (Kal tys)).
+
+(*********************************************************************************)
+(** *** Renamings. *)
+(*********************************************************************************)
+
+(** A renaming on terms is a function [nat -> nat] which is applied
+    to all free variables. *)
+Definition ren := nat -> nat.
+
+(** The identity renaming. *)
+Definition rid : ren := fun i => i.
+
+(** [rshift k] shifts indices by [k]. *)
+Definition rshift (k : nat) : ren := fun i => k + i.
+
+(** Cons an index with a renaming. *)
+Equations rcons (i0 : nat) (r : ren) : ren :=
+rcons i0 _ 0 := i0 ;
+rcons i0 r (S i) := r i.
+
+(** Compose two renamings (left to right composition). *)
+Definition rcomp (r1 r2 : ren) : ren :=
+  fun i => r2 (r1 i).
+
+(** Lift a renaming through a binder. *)
+Definition up_ren (r : ren) : ren := 
+  rcons 0 (rcomp r (rshift 1)).
+ 
+(** Rename a term. *)
+Equations rename {k} (t : expr k) (r : ren) : expr k :=
+rename (T_var i) r := T_var (r i) ;
+rename (T_ctor c al) r := T_ctor c (rename al r) ;
+rename T_al_nil r := T_al_nil ;
+rename (T_al_cons a al) r := T_al_cons (rename a r) (rename al r) ;
+rename (T_abase b x) r := T_abase b x ;
+rename (T_aterm t) r := T_aterm (rename t r) ;
+rename (T_abind a) r := T_abind (rename a (up_ren r)).
+
+(*********************************************************************************)
+(** *** Substitutions. *)
+(*********************************************************************************)
+
+(** A substitution on terms is a function [nat -> term] which is applied 
+    to all free variables. *)
+Definition subst := nat -> term.
+
+(** The identity substitution. *)
+Definition sid : subst := fun i => T_var i.
+
+(** [sshift k] shifts indices by [k]. *)
+Definition sshift (k : nat) : subst := 
+  fun i => T_var (k + i).
+
+(** Cons a expr with a substitution. *)
+Equations scons (t : term) (s : subst) : subst :=
+scons t s 0 := t ;
+scons t s (S i) := s i.
+
+(** Lift a substitution through a binder. *)
+Definition up_subst (s : subst) : subst :=
+  scons (T_var 0) (fun i => rename (s i) (rshift 1)).
+
+(** Apply a substitution to a expr. *)
+Equations substitute {k} (t : expr k) (s : subst) : expr k :=
+substitute (T_var i) s := s i ;
+substitute (T_ctor c al) s := T_ctor c (substitute al s) ;
+substitute T_al_nil s := T_al_nil ;
+substitute (T_al_cons a al) s := T_al_cons (substitute a s) (substitute al s) ;
+substitute (T_abase b x) s := T_abase b x ;
+substitute (T_aterm t) s := T_aterm (substitute t s) ;
+substitute (T_abind a) s := T_abind (substitute a (up_subst s)).
+
+(** Left to right composition of substitutions. *)
+Definition scomp (s1 s2 : subst) : subst :=
+  fun i => substitute (s1 i) s2.
+
+(*********************************************************************************)
+(** *** Setoid Rewrite Support. *)
+(*********************************************************************************)
+
+#[global] Instance up_ren_proper : Proper (point_eq ==> point_eq) up_ren.
+Proof. 
+intros r1 r2 Hr i. destruct i ; cbv [rcons up_ren rcomp].
+- reflexivity.
+- now rewrite Hr.
+Qed. 
+
+#[global] Instance rcons_proper : Proper (eq ==> point_eq ==> point_eq) rcons.
+Proof. 
+intros i1 i2 it s1 s2 Hs i. dependent elimination i ; simp rcons.
+now rewrite Hs. 
+Qed.
+
+#[global] Instance rcomp_proper n m o : Proper (point_eq ==> point_eq ==> point_eq) (@rcomp n m o).
+Proof. 
+intros s1 s2 Hs r1 r2 Hr i. dependent elimination i ; simp rcomp.
+- now rewrite Hs, Hr.
+- now rewrite Hs, Hr.
+Qed.
+
+#[global] Instance rename_proper n m k :
+  Proper (eq ==> point_eq ==> eq) (@rename n m k).
+Proof.
+intros t _ <- r1 r2 Hr. funelim (rename t _) ; simp rename in * ; auto.
+f_equal. apply H. now rewrite Hr.
+Qed.
+
+#[global] Instance up_subst_proper n m : Proper (point_eq ==> point_eq) (@up_subst n m).
+Proof.
+intros s1 s2 Hs i. dependent elimination i ; simp up_subst scons.
+- reflexivity.
+- now rewrite Hs.
+Qed. 
+
+#[global] Instance scons_proper n m : Proper (eq ==> point_eq ==> point_eq) (@scons n m).
+Proof. 
+intros t1 t2 Ht s1 s2 Hs i. 
+dependent elimination i ; simp scons. now rewrite Hs. 
+Qed.
+    
+#[global] Instance substitute_proper n m k : 
+  Proper (eq ==> point_eq ==> eq) (@substitute n m k).
+Proof. 
+intros t ? <- s1 s2 Hs. funelim (substitute t _) ; simp substitute in * ; auto.
+f_equal. apply H. now rewrite Hs.
+Qed. 
+
+#[global] Instance scomp_proper n m o : Proper (point_eq ==> point_eq ==> point_eq) (@scomp n m o).
+Proof. 
+intros s1 s2 Hs r1 r2 Hr i. dependent elimination i ; simp scomp.
+- now rewrite Hs, Hr.
+- now rewrite Hs, Hr.
+Qed.
+
+(*********************************************************************************)
+(** *** Properties of substitution. *)
+(*********************************************************************************)
+
+Lemma up_ren_comp {n m o} (r1 : ren n m) (r2 : ren m o) : 
+  rcomp (up_ren r1) (up_ren r2) =₁ up_ren (rcomp r1 r2).
+Proof. intros i. dependent elimination i ; reflexivity. Qed.  
+
+Lemma ren_ren {n m o k} (t : expr k n) (r1 : ren n m) (r2 : ren m o) : 
+  rename (rename t r1) r2 = rename t (rcomp r1 r2).
+Proof.
+funelim (rename t _) ; simp rename in * ; auto.
+now rewrite H, up_ren_comp.
+Qed.
+
+Lemma subst_ren {n m o k} (t : expr k n) (s : subst n m) (r : ren m o) : 
+  rename (substitute t s) r = substitute t (fun i => rename (s i) r).
+Proof.
+funelim (substitute t _) ; simp rename substitute in * ; auto.
+f_equal. rewrite H. apply substitute_proper ; auto.
+intros i. dependent elimination i ; simp up_subst scons rename ; auto.
+rewrite ren_ren, ren_ren. apply rename_proper ; auto.
+reflexivity.
+Qed.
+
+Lemma ren_subst {n m o k} (t : expr k n) (r : ren n m) (s : subst m o) : 
+  substitute (rename t r) s = substitute t (fun i => s (r i)).
+Proof.
+funelim (rename t r) ; simp rename substitute in * ; auto.
+f_equal. rewrite H. apply substitute_proper ; auto.
+intros i. dependent elimination i ; reflexivity.
+Qed.
+
+Lemma up_subst_comp {n m o} (s1 : subst n m) (s2 : subst m o) : 
+  scomp (up_subst s1) (up_subst s2) =₁ up_subst (scomp s1 s2).
+Proof. 
+intros i. dependent elimination i ; simp up_subst scomp scons substitute ; auto.
+rewrite ren_subst, subst_ren. apply substitute_proper ; auto.
+intros i. simp scons rshift fin_weaken. reflexivity.
+Qed.
+
+Lemma subst_subst {n m o k} (t : expr k n) (s1 : subst n m) (s2 : subst m o) : 
+  substitute (substitute t s1) s2 = substitute t (scomp s1 s2).
+Proof.
+funelim (substitute t _) ; simp substitute in * ; auto.
+f_equal. rewrite H. now rewrite up_subst_comp.
+Qed.
+
+Lemma up_subst_sid : (up_subst (@sid n)) =₁ sid.
+Proof. intros i ; dependent elimination i ; reflexivity. Qed.
+#[global] Hint Rewrite @up_subst_sid : up_subst.
+
+Lemma subst_sid {n k} (t : expr n k) : substitute t sid = t.
+Proof.
+induction t ; simp substitute in * ; auto.
+rewrite up_subst_sid. auto.
+Qed.
+#[global] Hint Rewrite @subst_sid : substitute.
+
+Lemma scomp_id_l (s : subst n m) : scomp sid s =₁ s.
+Proof. reflexivity. Qed.
+#[global] Hint Rewrite @scomp_id_l : scomp.
+
+Lemma scomp_id_r (s : subst n m) : scomp s sid =₁ s.
+Proof. intros i. simp scomp substitute. reflexivity. Qed.
+#[global] Hint Rewrite @scomp_id_r : scomp.
+
+Lemma scomp_assoc {n m o p} (s1 : subst n m) (s2 : subst m o) (s3 : subst o p) : 
+  scomp (scomp s1 s2) s3 =₁ scomp s1 (scomp s2 s3).
+Proof. intros i. simp scomp. now rewrite subst_subst. Qed.
+
+Lemma ren_is_subst {n m k} (t : expr k n) (r : ren n m) : 
+  rename t r = substitute t (fun i => T_var (r i)).
+Proof.
+funelim (rename t r) ; simp rename substitute in * ; auto.
+f_equal. rewrite H. apply substitute_proper ; auto.
+intros i. dependent elimination i ; reflexivity.
+Qed.
+
+Lemma rshift_sshift {n k} (t : expr k n) : 
+  rename t (rshift 1) = substitute t (sshift 1).
+Proof. rewrite ren_is_subst. reflexivity. Qed.
+    
+Lemma up_subst_alt (s : subst n m) :
+  up_subst s =₁ scons (T_var fin_zero) (scomp s (sshift 1)).
+Proof.
+simp up_subst. apply scons_proper ; auto.
+intros i. simp scomp. now rewrite rshift_sshift.
+Qed.
+
+Lemma sshift_succ_r k : sshift (S k) =₁ scomp (@sshift n k) (sshift 1).
+Proof. intros i. dependent elimination i ; reflexivity. Qed.    
+
+Lemma sid_scons : scons (T_var fin_zero) (sshift 1) =₁ @sid (S n).
+Proof. intros i. dependent elimination i ; reflexivity. Qed.
+#[global] Hint Rewrite @sid_scons : scons.
+
+Lemma scomp_scons_distrib {n m o} (t : term m) (s1 : subst n m) (s2 : subst m o) :
+  scomp (scons t s1) s2 =₁ scons (substitute t s2) (scomp s1 s2).
+Proof. intros i. dependent elimination i ; reflexivity. Qed.
+
+End Make.
